cleanup

theories/FOL/Util/FA_facts.v
@@ -5,184 +5,6 @@ Import Vector.VectorNotations.
 
 
 
-Lemma bounded_S_exists N phi : bounded (S N) phi <-> bounded N (∃ phi).
-Proof.
-  split; intros H.
-  - now constructor.
-  - inversion H. apply inj_pair2_eq_dec' in H4 as ->; trivial.
-    unfold Dec.dec. decide equality.
-Qed.
-
-Lemma bounded_S_forall N phi : bounded (S N) phi <-> bounded N (∀ phi).
-Proof.
-  split; intros H.
-  - now constructor.
-  - inversion H. apply inj_pair2_eq_dec' in H4 as ->; trivial.
-    unfold Dec.dec. decide equality.
-Qed.
-
-
-
-Section ND.
-
-  Variable p : peirce.
-
-
-  Fixpoint iter {X: Type} f n (x : X) :=
-    match n with
-      0 => x
-    | S m => f (iter f m x)
-    end.
-
-  Fact iter_switch {X} f n x : f (@iter X f n x) = iter f n (f x).
-  Proof. induction n; cbn; now try rewrite IHn. Qed.
-    
-  
-  Lemma subst_up_var k x sigma : x < k -> (var x)`[iter up k sigma] = var x.
-  Proof.
-    induction k in x, sigma |-*.
-    - now intros ?%PeanoNat.Nat.nlt_0_r.
-    - intros H.
-      destruct (Compare_dec.lt_eq_lt_dec x k) as [[| <-]|].
-      + cbn [iter]. rewrite iter_switch. now apply IHk.
-      + destruct x. reflexivity.
-        change (iter _ _ _) with (up (iter up (S x) sigma)).
-        change (var (S x)) with ((var x)`[↑]).
-        rewrite up_term, IHk. reflexivity. constructor.
-      + lia.
-  Qed.
-  
-  
-  Lemma subst_bounded_term t sigma k : bounded_t k t -> t`[iter up k sigma] = t.
-  Proof.
-    induction 1.
-    - now apply subst_up_var.
-    - cbn. f_equal.
-      rewrite <-(Vector.map_id _ _ v) at 2.
-      apply Vector.map_ext_in. auto.
-  Qed.
-  
-
-  Lemma subst_bounded k phi sigma : bounded k phi -> phi[iter up k sigma] = phi.
-  Proof.
-    induction 1 in sigma |-*; cbn.
-    - f_equal.
-      rewrite <-(Vector.map_id _ _ v) at 2.
-      apply Vector.map_ext_in.
-      intros t Ht. apply subst_bounded_term. auto.
-    - now rewrite IHbounded1, IHbounded2.
-    - f_equal.
-      change (up _) with (iter up (S n) sigma).
-      apply IHbounded.
-    - reflexivity.
-  Qed.
-
-
-  Definition exist_times n (phi : form) := iter (fun psi => ∃ psi) n phi.
-  Definition forall_times n (phi : form) := iter (fun psi => ∀ psi) n phi.
-  
-
-  Lemma up_decompose sigma phi : phi[up (S >> sigma)][(sigma 0)..] = phi[sigma].
-  Proof.
-    rewrite subst_comp. apply subst_ext.
-    intros [].
-    - reflexivity.
-    - apply subst_term_shift.
-  Qed.  
-  
-  
-  Lemma subst_exist_prv {sigma N Gamma} phi :
-    Gamma ⊢ phi[sigma] -> bounded N phi -> Gamma ⊢ exist_times N phi. 
-  Proof.
-    induction N in phi, sigma |-*; intros; cbn.
-    - erewrite <-(subst_bounded 0); eassumption.
-    - rewrite iter_switch. eapply (IHN (S >> sigma)).
-      cbn. eapply (ExI (sigma 0)).
-      now rewrite up_decompose.
-      now apply bounded_S_exists.
-  Qed.
-
-  
-  Lemma subst_forall_prv phi {N Gamma} :
-    Gamma ⊢ (iter (fun psi => ∀ psi) N phi) -> bounded N phi -> forall sigma, Gamma ⊢ phi[sigma].
-  Proof.
-    induction N in phi |-*; intros ?? sigma; cbn in *.
-    - change sigma with (iter up 0 sigma).
-      now rewrite (subst_bounded 0).
-    - specialize (IHN (∀ phi) ).
-      rewrite <-up_decompose.
-      apply AllE. apply IHN.
-      now rewrite <-iter_switch.
-      now apply bounded_S_forall.
-  Qed.
-
-End ND.
-
-
-Section SEM.
-
-
-  Context {D : Type}.
-  Context {I : interp D}.
-
-  
-  Lemma bounded_eval_t n t sigma tau :
-    (forall k, n > k -> sigma k = tau k) -> bounded_t n t -> eval sigma t = eval tau t.
-  Proof.
-    intros H. induction 1; cbn; auto.
-    f_equal. now apply Vector.map_ext_in.
-  Qed.
-
-  
-  Lemma bound_ext N phi rho sigma :
-    bounded N phi -> (forall n, n < N -> rho n = sigma n) -> (rho ⊨ phi <-> sigma ⊨ phi).
-  Proof.
-    induction 1 in sigma, rho |- *; cbn; intros HN; try tauto.
-    - enough (map (eval rho) v = map (eval sigma) v) as E. now setoid_rewrite E.
-      apply Vector.map_ext_in. intros t Ht.
-      eapply bounded_eval_t; try apply HN. now apply H.
-    - destruct binop; now rewrite (IHbounded1 rho sigma), (IHbounded2 rho sigma).
-    - destruct quantop.
-      + split; intros Hd d; eapply IHbounded.
-        all : try apply (Hd d); intros [] Hk; cbn; auto.
-        symmetry. all: apply HN; lia.
-      + split; intros [d Hd]; exists d; eapply IHbounded.
-        all : try apply Hd; intros [] Hk; cbn; auto.
-        symmetry. all: apply HN; lia.
-  Qed.
-  
-
-  Corollary sat_closed rho sigma phi :
-    bounded 0 phi -> rho ⊨ phi <-> sigma ⊨ phi.
-  Proof.
-    intros H. eapply bound_ext. apply H. lia.
-  Qed.
-
-  
-  Lemma subst_exist_sat rho phi N :
-    rho ⊨ phi -> bounded N phi -> forall rho, rho ⊨ (exist_times N phi).  
-  Proof.
-    induction N in phi, rho |-*; intros.
-    - cbn. eapply sat_closed; eassumption.
-    - cbn -[sat]. rewrite iter_switch. apply (IHN (S >> rho)).
-      exists (rho 0). eapply sat_ext. 2: apply H.
-      now intros [].
-      now apply bounded_S_exists.
-  Qed.
-  
-
-  Fact subst_exist_sat2 N : forall rho phi, rho ⊨ (exist_times N phi) -> (exists sigma, sigma ⊨ phi).
-  Proof.
-    induction N.
-    - eauto.
-    - intros rho phi [? H]. now apply IHN in H.
-  Qed.
-  
-
-End SEM.
-
-
-
 Section FA_prv.
 
   Variable p : peirce.
@@ -209,7 +31,7 @@ Section FA_prv.
     pose (sigma := [t] ∗ var ).
     change (FAeq ⊢ _) with (FAeq ⊢ ($0 == $0)[sigma]).
     
-    eapply (@subst_forall_prv _ _ 1).
+    eapply subst_forall_prv with 1.
     apply Ctx. all : firstorder. constructor.
     repeat solve_bounds.
   Qed.
@@ -222,7 +44,7 @@ Section FA_prv.
     pose (sigma := [x ; y] ∗ var ).
     change (FAeq ⊢ _) with (FAeq ⊢ ($1 == $0 ~> $0 == $1)[sigma]).
     
-    apply (@subst_forall_prv _ _ 2).
+    eapply subst_forall_prv with 2.
     apply Ctx. all : firstorder.
     repeat solve_bounds.
   Qed.
@@ -237,7 +59,7 @@ Section FA_prv.
     pose (sigma := [x ; y ; z] ∗ var).
     change (FAeq ⊢ _) with (FAeq ⊢ ($2 == $1 ~> $1 == $0 ~> $2 == $0)[sigma]).
     
-    apply (@subst_forall_prv _ _ 3).
+    eapply subst_forall_prv with 3.
     apply Ctx. all : try firstorder.
     repeat solve_bounds.
   Qed.
@@ -250,7 +72,7 @@ Section FA_prv.
     pose (sigma := [y ; x] ∗ var ).
     change (FAeq ⊢ _) with (FAeq ⊢ ($0 == $1 ~> σ $0 == σ $1)[sigma]).
 
-    apply (@subst_forall_prv _ _ 2).
+    eapply subst_forall_prv with 2.
     apply Ctx. all : firstorder.
     repeat solve_bounds.
   Qed.
@@ -265,7 +87,7 @@ Section FA_prv.
     pose (sigma := [y2 ; y1 ; x2 ; x1] ∗ var).
     change (FAeq ⊢ _) with (FAeq ⊢ ($0 == $1 ~> $2 == $3 ~> $0 ⊕ $2 == $1 ⊕ $3)[sigma]).
 
-    apply (@subst_forall_prv _ _ 4).
+    eapply subst_forall_prv with 4.
     apply Ctx. all: firstorder.
     repeat solve_bounds.
   Qed.
@@ -280,7 +102,7 @@ Section FA_prv.
     pose (sigma := [y2 ; y1 ; x2 ; x1] ∗ var).
     change (FAeq ⊢ _) with (FAeq ⊢ ($0 == $1 ~> $2 == $3 ~> $0 ⊗ $2 == $1 ⊗ $3)[sigma]).
     
-    apply (@subst_forall_prv _ _ 4).
+    eapply subst_forall_prv with 4.
     apply Ctx. all: firstorder.
     repeat solve_bounds.
   Qed.
@@ -293,7 +115,7 @@ Section FA_prv.
     pose (sigma := [y ; x] ∗ var).
     change (FAeq ⊢ _) with (FAeq ⊢ (σ $0 ⊕ $1 == σ ($0 ⊕ $1))[sigma]).
 
-    apply (@subst_forall_prv _ _ 2).
+    eapply subst_forall_prv with 2.
     apply Ctx. all : firstorder.
     repeat solve_bounds.
   Qed.
@@ -325,7 +147,7 @@ Section FA_prv.
     pose (sigma := [x ; y] ∗ var).
     change (FAeq ⊢ _) with (FAeq ⊢ ((σ $1) ⊗ $0 == $0 ⊕ ($1 ⊗ $0))[sigma]).
 
-    eapply (@subst_forall_prv _ _ 2).
+    eapply subst_forall_prv with 2.
     apply Ctx. all : firstorder.
     repeat solve_bounds.
   Qed.
