theories/FOL/FSAT.v
@@ -4,7 +4,7 @@ Require Import List.
  
 (* ** Syntax as defined in Util/Syntax.v 
 
- Inductive term  : Type :=
+  Inductive term  : Type :=
   | var : nat -> term
   | func : forall (f : syms), vec term (ar_syms f) -> term.
 
@@ -21,14 +21,22 @@ Require Import List.
 
 Existing Instance falsity_on.
 
+(* Definition of finiteness *)
+
 Definition listable X :=
   exists L, forall x : X, In x L.
+
+(* Satisfiability in a finite and decidable model *)
 
 Definition FSAT (phi : form) :=
   exists D (I : interp D) rho, listable D /\ decidable (fun v => i_atom (P:=tt) v) /\ rho ⊨ phi.
 
+(* Satisfiability in a discrete, finite, and decidable model *)
+
 Definition FSATd (phi : form) :=
   exists D (I : interp D) rho, listable D /\ discrete D /\ decidable (fun v => i_atom (P:=tt) v) /\ rho ⊨ phi.
+
+(* Satisfiability in a discrete, finite, and decidable model restricted to closed formulas *)
 
 Definition cform := { phi | bounded 0 phi }.
 
